program_logic/ectx_language.v
@@ -1,0 +1,112 @@
+From iris.algebra Require Export base.
+From iris.program_logic Require Export language.
+
+(* We need to make thos arguments indices that we want canonical structure
+   inference to use a keys. *)
+Class ectx_language (expr val ectx state : Type) := EctxLanguage {
+  of_val : val → expr;
+  to_val : expr → option val;
+  empty_ectx : ectx;
+  comp_ectx : ectx → ectx → ectx;
+  fill : ectx → expr → expr;
+  atomic : expr → Prop;
+  head_step : expr → state → expr → state → option expr → Prop;
+
+  to_of_val v : to_val (of_val v) = Some v;
+  of_to_val e v : to_val e = Some v → of_val v = e;
+  val_stuck e1 σ1 e2 σ2 ef : head_step e1 σ1 e2 σ2 ef → to_val e1 = None;
+
+  fill_empty e : fill empty_ectx e = e;
+  fill_comp K1 K2 e : fill K1 (fill K2 e) = fill (comp_ectx K1 K2) e;
+  fill_inj K e1 e2 : fill K e1 = fill K e2 → e1 = e2;
+  fill_not_val K e : to_val e = None → to_val (fill K e) = None;
+
+  step_by_val K K' e1 e1' σ1 e2 σ2 ef :
+    fill K e1 = fill K' e1' →
+    to_val e1 = None →
+    head_step e1' σ1 e2 σ2 ef →
+    exists K'', K' = comp_ectx K K'';
+
+  atomic_not_val e : atomic e → to_val e = None;
+  atomic_step e1 σ1 e2 σ2 ef :
+    atomic e1 →
+    head_step e1 σ1 e2 σ2 ef →
+    is_Some (to_val e2);
+  atomic_fill e K :
+    atomic (fill K e) →
+    to_val e = None →
+    K = empty_ectx;
+}.
+Arguments of_val {_ _ _ _ _} _.
+Arguments to_val {_ _ _ _ _} _.
+Arguments empty_ectx {_ _ _ _ _}.
+Arguments comp_ectx {_ _ _ _ _} _ _.
+Arguments fill {_ _ _ _ _} _ _.
+Arguments atomic {_ _ _ _ _} _.
+Arguments head_step {_ _ _ _ _} _ _ _ _ _.
+
+Arguments to_of_val {_ _ _ _ _} _.
+Arguments of_to_val {_ _ _ _ _} _ _ _.
+Arguments val_stuck {_ _ _ _ _} _ _ _ _ _ _.
+Arguments fill_empty {_ _ _ _ _} _.
+Arguments fill_comp {_ _ _ _ _} _ _ _.
+Arguments fill_inj {_ _ _ _ _} _ _ _ _.
+Arguments fill_not_val {_ _ _ _ _} _ _ _.
+Arguments step_by_val {_ _ _ _ _} _ _ _ _ _ _ _ _ _ _ _.
+Arguments atomic_not_val {_ _ _ _ _} _ _.
+Arguments atomic_step {_ _ _ _ _} _ _ _ _ _ _ _.
+Arguments atomic_fill {_ _ _ _ _} _ _ _ _.
+
+(* From an ectx_language, we can construct a language. *)
+Section Language.
+  Context {expr val ectx state : Type} (Λ : ectx_language expr val ectx state).
+  Implicit Types (e : expr) (K : ectx).
+
+  Inductive prim_step (e1 : expr) (σ1 : state)
+    (e2 : expr) (σ2: state) (ef: option expr) : Prop :=
+  Ectx_step K e1' e2' :
+    e1 = fill K e1' → e2 = fill K e2' →
+    head_step e1' σ1 e2' σ2 ef → prim_step e1 σ1 e2 σ2 ef.
+
+  Lemma val_prim_stuck e1 σ1 e2 σ2 ef :
+    prim_step e1 σ1 e2 σ2 ef → to_val e1 = None.
+  Proof. intros [??? -> -> ?]; eauto using fill_not_val, val_stuck. Qed.
+
+  Lemma atomic_prim_step e1 σ1 e2 σ2 ef :
+  atomic e1 → prim_step e1 σ1 e2 σ2 ef → is_Some (to_val e2).
+  Proof.
+    intros Hatomic [K e1' e2' -> -> Hstep].
+    assert (K = empty_ectx) as -> by eauto 10 using atomic_fill, val_stuck.
+    eapply atomic_step; first done. by rewrite !fill_empty.
+  Qed.
+
+  Canonical Structure ectx_lang : language := {|
+    language.expr := expr; language.val := val; language.state := state;
+    language.of_val := of_val; language.to_val := to_val;
+    language.atomic := atomic; language.prim_step := prim_step;
+    language.to_of_val := to_of_val; language.of_to_val := of_to_val;
+    language.val_stuck := val_prim_stuck; language.atomic_not_val := atomic_not_val;
+    language.atomic_step := atomic_prim_step
+  |}.
+
+  (* Every evaluation context is a context. *)
+  Global Instance ectx_lang_ctx K : LanguageCtx ectx_lang (fill K).
+  Proof.
+    split.
+    - eauto using fill_not_val.
+    - intros ????? [K' e1' e2' Heq1 Heq2 Hstep].
+      by exists (comp_ectx K K') e1' e2'; rewrite ?Heq1 ?Heq2 ?fill_comp.
+    - intros e1 σ1 e2 σ2 ? Hnval [K'' e1'' e2'' Heq1 -> Hstep].
+      destruct (step_by_val K K'' e1 e1'' σ1 e2'' σ2 ef) as [K' ->]; eauto.
+      rewrite -fill_comp in Heq1; apply fill_inj in Heq1.
+      exists (fill K' e2''); rewrite -fill_comp; split; auto.
+      econstructor; eauto.
+  Qed.
+End Language.
+  
+
+
+
+
+
+  
